theory/Util/Loop.v
@@ -13,26 +13,84 @@ Record loop_data (X : Type) : Type := {
   measure : X -> nat;
   step : X -> X;
 
-  step_measure : forall x, measure (step x) <= measure x
+  measure_bound : exists B, forall x, measure x <= B;
+
+  step_measure : forall x, measure x <= measure (step x)
   }.
 
 Arguments measure {_} _ _.
 Arguments step {_} _ _.
 
 Arguments step_measure {_} _ _.
+Arguments measure_bound {_} _.
+
+Definition rel {X} (l : loop_data X) : X -> X -> Prop :=
+  fun a b => measure l b < measure l a.
+
+Fixpoint acc_contra {X} (R S : X -> X -> Prop)
+  (f : forall x y, R x y -> S x y) {x}
+  (a : Acc S x) {struct a} : Acc R x.
+Proof.
+  destruct a as [accs].
+  constructor.
+  intros y r.
+  apply f in r.
+  apply accs in r.
+  apply (acc_contra _ _ _ f).
+  exact r.
+Defined.
+
+Lemma wf_impl {X} (R S : X -> X -> Prop) :
+  (forall x y, R x y -> S x y) ->
+  well_founded S ->
+  well_founded R.
+Proof.
+  intros RS HS x.
+  specialize (HS x).
+  exact (acc_contra R S RS HS).
+Qed.
+
+Fixpoint acc_func {X Y} (f : X -> Y)
+  (R : Y -> Y -> Prop) {x} (a : Acc R (f x))
+  {struct a} : Acc (fun x1 x2 => R (f x1) (f x2)) x.
+Proof.
+  destruct a.
+  constructor.
+  intros x' Rx.
+  apply H in Rx.
+  apply acc_func in Rx.
+  auto.
+Qed.
+
+Lemma wf_func {X Y} (f : X -> Y)
+  (R : Y -> Y -> Prop) (R_wf : well_founded R) :
+  well_founded (fun x x' => R (f x) (f x')).
+Proof.
+  intro x.
+  apply acc_func.
+  apply R_wf.
+Qed.
+
+Lemma rel_wf {X} (l : loop_data X) : well_founded (rel l).
+Proof.
+  destruct (measure_bound l) as [B HB].
+  apply wf_impl with (S := fun n m => measure l m < measure l n <= B).
+  - intros; split; auto.
+  - apply (wf_func (measure l) (fun a b => b < a <= B)).
+    apply PeanoNat.Nat.gt_wf.
+Qed.
 
 Fixpoint loop_aux {X} (l : loop_data X) (x : X)
-  (a : Acc (Wf_nat.ltof _ (measure l)) x) {struct a} : X :=
-  match le_lt_eq_dec _ _ (step_measure l x) with
-  | left pf =>
-    match a with
-    | Acc_intro _ accs => loop_aux l (step l x) (accs _ pf)
-    end
-  | right _ => x
-  end.
+  (a : Acc (rel l) x) {struct a} : X.
+  destruct (le_lt_eq_dec _ _ (step_measure l x)).
+  - destruct a as [accs].
+    apply (loop_aux _ l (step l x)).
+    apply accs. exact l0.
+  - exact x.
+Defined.
 
 Fixpoint loop_aux_ext {X} (l : loop_data X) (x : X)
-  (a : Acc (Wf_nat.ltof _ (measure l)) x) {struct a} :
+  (a : Acc (rel l) x) {struct a} :
   forall a',
   loop_aux l x a = loop_aux l x a'.
 Proof.
@@ -42,8 +100,11 @@ Proof.
   - reflexivity.
 Defined.
 
-Definition loop {X} (l : loop_data X) (x : X) : X :=
-  loop_aux l x (Wf_nat.well_founded_ltof X (measure l) x).
+Definition loop {X} (l : loop_data X) (x : X) : X.
+  apply (
+  loop_aux l x).
+  apply rel_wf.
+Defined.
 
 Lemma loop_eq {X} (l : loop_data X) (x : X) :
   loop l x =
@@ -54,7 +115,7 @@ Lemma loop_eq {X} (l : loop_data X) (x : X) :
 Proof.
   unfold loop at 1.
   unfold loop_aux.
-  destruct (Wf_nat.well_founded_ltof X (measure l) x).
+  destruct (rel_wf l x).
   - destruct (le_lt_eq_dec).
     + unfold loop.
       unfold loop_aux.
@@ -65,15 +126,16 @@ Defined.
 Lemma loop_measure_aux {X} (l : loop_data X) : forall n x, n = measure l x ->
   measure l (loop l x) = measure l (step l (loop l x)).
 Proof.
+  destruct (measure_bound l) as [B HB].
   intro n.
-  induction (Wf_nat.lt_wf n) as [n _ IHn].
+  induction (PeanoNat.Nat.gt_wf B n) as [n _ IHn].
   intros.
   rewrite loop_eq.
   destruct le_lt_eq_dec.
   - rewrite (IHn (measure l (step l x))); [reflexivity| |reflexivity].
     rewrite H.
-    pose (step_measure l x). lia.
-  - symmetry; exact e.
+    split; auto.
+  - symmetry; auto.
 Qed.
 
 Lemma loop_measure {X} (l : loop_data X) : forall x,
@@ -83,31 +145,19 @@ Proof.
   eapply loop_measure_aux; reflexivity.
 Qed.
 
-Lemma loop_iter_aux {X} (l : loop_data X) : forall n x, n = measure l x ->
-  {n : nat & loop l x = Nat.iter n (step l) x}.
-Proof.
-  intro n.
-  induction (Wf_nat.lt_wf n) as [n _ IHn].
-  intros.
-  rewrite loop_eq.
-  destruct le_lt_eq_dec.
-  - assert (pf : measure l (step l x) < n).
-    { rewrite H.
-      pose proof (step_measure l x); lia.
-    }
-    destruct (IHn (measure l (step l x)) pf (step l x) eq_refl) as [k Hk].
-    exists (S k).
-    rewrite Hk.
-    simpl.
-    apply iter_lemma.
-  - exists 0; reflexivity.
-Defined.
-
 Lemma loop_iter {X} (l : loop_data X) : forall x,
   {n : nat & loop l x = Nat.iter n (step l) x}.
 Proof.
   intro x.
-  exact (loop_iter_aux l (measure l x) x eq_refl).
+  induction (rel_wf l x) as [x _ IHx].
+  rewrite loop_eq.
+  destruct le_lt_eq_dec.
+  - destruct (IHx (step l x)) as [n Hn].
+    + auto.
+    + exists (S n).
+      simpl; rewrite Hn.
+      apply iter_lemma.
+  - exists 0; reflexivity.
 Defined.
 
 Record validity_data {X} (l : loop_data X) : Type := {
